src/InformationOrdering.v
@@ -1,0 +1,479 @@
+(** * Information ordering and observable equivalence *)
+
+Require Import Coq.Program.Basics.
+Require Import Coq.Setoids.Setoid.
+Require Import Coq.Classes.RelationClasses.
+Require Import Coq.Classes.Morphisms.
+Require Import Coq.Classes.Morphisms_Prop.
+Require Export Codes.
+Open Scope code_scope.
+
+Definition code_le {Var : Set} (x y : Code Var) :=
+  forall (Var' : Set) (c : Code Var') (f : Var -> Code Var'),
+  conv (c * (x @ f)) -> conv (c * (y @ f)).
+Notation "x [= y" := (code_le x y)%code : code_scope.
+
+Definition code_eq {Var : Set} (x y : Code Var) := x [= y /\ y [= x.
+Notation "x == y" := (code_eq x y)%code : code_scope.
+
+Instance code_le_eq_subrelation (Var : Set) :
+  subrelation (@code_eq Var) (@code_le Var).
+Proof.
+  unfold subrelation, predicate_implication, pointwise_lifting.
+  unfold code_eq; intros x y [xy yx]; auto.
+Qed.
+
+Instance code_le_beta_proper (Var : Set) :
+  Proper (beta ==> beta ==> iff) (@code_le Var).
+Proof.
+  intros x x' Hx y y' Hy; split; unfold code_le; intros Hle Var' c f Hc.
+    rewrite <- Hy; apply Hle; rewrite -> Hx; auto.
+  rewrite -> Hy; apply Hle; rewrite <- Hx; auto.
+Qed.
+
+Instance code_eq_beta_proper (Var : Set) :
+  Proper (beta ==> beta ==> iff) (@code_eq Var).
+Proof.
+  unfold code_eq.
+  intros x x' xx' y y' yy'; split; intros [xy yx].
+    split; rewrite <- xx'; rewrite <- yy'; auto.
+  split; rewrite -> xx'; rewrite -> yy'; auto.
+Qed.
+
+Lemma code_le_beta (Var : Set) (x y : Code Var) : beta x y -> x [= y.
+Proof.
+  unfold code_le; intros H Var' c f Hc.
+  rewrite <- H; auto.
+Qed.
+Hint Resolve code_le_beta.
+
+Instance code_le_beta_subrelation (Var : Set) :
+  subrelation beta code_le := code_le_beta Var.
+
+Lemma code_eq_beta (Var : Set) (x y : Code Var) : beta x y -> x == y.
+Proof.
+  unfold code_le; intro H; split; intros Var' c f Hc.
+  rewrite <- H; auto.
+  rewrite -> H; auto.
+Qed.
+Hint Resolve code_eq_beta.
+
+Instance code_eq_beta_subrelation (Var : Set) :
+  subrelation beta code_eq := code_eq_beta Var.
+
+Instance code_le_pi_proper (Var : Set) :
+  Proper (pi ++> pi --> impl) (@code_le Var).
+Proof.
+  intros x x' Hx y y' Hy; unfold code_le; intros Hle Var' c f Hc.
+  unfold flip in *.
+  rewrite (pi_ap_right (code_sub_pi_right _ _ _ _ _ Hy)).
+  apply Hle. rewrite -> Hx. auto.
+Qed.
+
+Instance code_le_pi_subrelation (Var : Set) :
+  subrelation (inverse pi) (@code_le Var).
+Proof.
+  unfold subrelation, predicate_implication, pointwise_lifting, flip.
+  intros x y H; unfold code_le; intros Var' c f Hc.
+  rewrite -> H; auto.
+Qed.
+
+Instance code_le_refl (Var : Set) : Reflexive (@code_le Var).
+Proof. unfold code_le; auto. Qed.
+
+Instance code_eq_refl (Var : Set) : Reflexive (@code_eq Var).
+Proof. simpl_relation. Qed.
+
+Instance code_le_trans (Var : Set) : Transitive (@code_le Var).
+Proof. unfold code_le; auto. Qed.
+
+Instance code_eq_trans (Var : Set) : Transitive (@code_eq Var).
+Proof.
+  unfold code_eq, code_le; simpl_relation.
+Qed.
+
+Instance code_eq_sym (Var : Set) : Symmetric (@code_eq Var).
+Proof.
+  unfold code_eq, code_le; simpl_relation.
+Qed.
+
+Instance code_le_preorder (Var : Set) : PreOrder (@code_le Var).
+Proof.
+  split; [apply code_le_refl | apply code_le_trans].
+Qed.
+
+Instance code_eq_equivalence (Var : Set) : Equivalence (@code_eq Var).
+Proof.
+  split; [apply code_eq_refl | apply code_eq_sym | apply code_eq_trans].
+Qed.
+
+Instance code_le_partialorder (Var : Set) :
+  PartialOrder (@code_eq Var) (@code_le Var).
+Proof. simpl_relation. Qed.
+
+Lemma code_le_ap_right (Var : Set) (x y y' : Code Var) :
+  y [= y' -> x * y [= x * y'.
+Proof.
+  unfold code_le, conv; intros H Var' c f.
+  repeat rewrite code_sub_ap.
+  intros Hconv.
+  rewrite <- (beta_ap_right beta_b); apply H.
+  rewrite -> (beta_ap_right beta_b); auto.
+Qed.
+Hint Resolve code_le_ap_right.
+
+Lemma code_le_ap_left (Var : Set) (x x' y : Code Var) :
+  x [= x' -> x * y [= x' * y.
+Proof.
+  unfold code_le, conv; intros H Var' c f.
+  repeat rewrite code_sub_ap.
+  intros Hconv.
+  rewrite <- (beta_ap_right (beta_ap_right (beta_ap_left beta_i))).
+  rewrite <- (beta_ap_right (beta_ap_right beta_c)).
+  rewrite <- (beta_ap_right beta_b).
+  apply H.
+  rewrite -> (beta_ap_right beta_b).
+  rewrite -> (beta_ap_right (beta_ap_right beta_c)).
+  rewrite -> (beta_ap_right (beta_ap_right (beta_ap_left beta_i))).
+  auto.
+Qed.
+Hint Resolve code_le_ap_left.
+
+Lemma code_le_ap (Var : Set) (x x' y y' : Code Var) :
+  x [= x' -> y [= y' -> x * y [= x' * y'.
+Proof.
+  intros Hx Hy; transitivity (x * y'); auto.
+Qed.
+Hint Resolve code_le_ap.
+
+Lemma code_eq_ap_right (Var : Set) (x y y' : Code Var) :
+  y == y' -> x * y == x * y'.
+Proof.
+  unfold code_eq; intros [H H']; split; auto.
+Qed.
+Hint Resolve code_eq_ap_right.
+
+Lemma code_eq_ap_left (Var : Set) (x x' y : Code Var) :
+  x == x' -> x * y == x' * y.
+Proof.
+  unfold code_eq; intros [H H']; split; auto.
+Qed.
+Hint Resolve code_eq_ap_left.
+
+Lemma code_eq_ap (Var : Set) (x x' y y' : Code Var) :
+  x == x' -> y == y' -> x * y == x' * y'.
+Proof.
+  intros Hx Hy; transitivity (x * y'); auto.
+Qed.
+Hint Resolve code_eq_ap.
+
+Instance code_ap_le (Var : Set) :
+  Proper (code_le ==> code_le ==> code_le) (@code_ap Var).
+Proof.
+  intros x x' Hx y y' Hy.
+  apply code_le_trans with (x * y'); auto.
+Qed.
+
+Instance code_ap_eq (Var : Set) :
+  Proper (code_eq ==> code_eq ==> code_eq) (@code_ap Var).
+Proof.
+  intros x x' Hx y y' Hy.
+  apply code_eq_trans with (x * y'); auto.
+Qed.
+
+Ltac code_le_monotonicity := repeat (
+  apply code_le_ap_left ||
+  apply code_le_ap_right ||
+  apply code_le_ap).
+
+Ltac code_eq_monotonicity := repeat (
+  apply code_eq_ap_left ||
+  apply code_eq_ap_right ||
+  apply code_eq_ap).
+
+Ltac monotonicity :=
+  match goal with
+  | [|- _ [= _] => code_le_monotonicity
+  | [|- _ == _] => code_eq_monotonicity
+  end.
+
+Instance code_abs_le (Var Var' : Set) (b : Var -> option Var') :
+  Proper (code_le ==> code_le) (code_abs b).
+Proof.
+  intros x x' Hx.
+Admitted.
+
+Instance code_abs_eq (Var Var' : Set) (b : Var -> option Var') :
+  Proper (code_eq ==> code_eq) (code_abs b).
+Proof.
+  intros x x' Hx.
+Admitted.
+
+Instance code_close_le (Var : Set) : Proper (code_le ==> code_le) (@close Var).
+Proof.
+  intros x x' xx'.
+Admitted.
+
+Instance code_close_eq (Var : Set) : Proper (code_eq ==> code_eq) (@close Var).
+Proof.
+  intros x x' xx'.
+Admitted.
+
+Lemma code_le_top (Var : Set) (x : Code Var) : x [= TOP.
+Proof.
+  unfold code_le, conv ; intros Var' c f Hred.
+  simpl.
+  rewrite <- beta_b.
+  rewrite -> (pi_top (x @ f)) at 1.
+  rewrite -> beta_b; auto.
+Qed.
+Hint Resolve code_le_top.
+
+Lemma code_le_bot (Var : Set) (x : Code Var) : BOT [= x.
+Proof.
+  unfold code_le, conv; intros Var' c f Hred.
+  rewrite <- beta_b.
+  rewrite -> (pi_ap_right (pi_bot _)).
+  rewrite -> beta_b; auto.
+Qed.
+Hint Resolve code_le_bot.
+
+(** *** Proving information ordering *)
+
+Lemma code_le_j_left (Var : Set) (x y : Code Var) : x [= x || y.
+Proof.
+  unfold code_le, conv; intros Var' c f Hred.
+  rewrite pi_j_left; auto.
+Qed.
+Hint Resolve code_le_j_left.
+
+Lemma code_le_j_right (Var : Set) (x y : Code Var) : y [= x || y.
+Proof.
+  unfold code_le, conv; intros Var' c f Hred.
+  rewrite pi_j_right; auto.
+Qed.
+Hint Resolve code_le_j_right.
+
+Lemma code_le_j_ub (Var : Set) (x y z : Code Var) :
+  x [= z -> y [= z -> x || y [= z.
+Proof.
+  unfold code_le, conv; intros Hx Hy Var' c f Hconv.
+Admitted.
+Hint Resolve code_le_j_ub.
+
+Lemma code_le_join (Var : Set) (x y z : Code Var) :
+  x || y [= z <-> x [= z /\ y [= z.
+Proof.
+  split; intro H.
+    split; apply code_le_trans with (x || y); auto.
+  destruct H as [Hx Hy]; auto.
+Qed.
+Hint Resolve code_le_join.
+
+Lemma code_le_eq_j (Var : Set) (x y : Code Var) : x [= y <-> y == y || x.
+Proof.
+  split; intro H; [split | rewrite H]; auto.
+Qed.
+
+Lemma code_le_j_idem (Var : Set) (x : Code Var) : x||x [= x.
+Proof.
+  apply code_le_join; split; reflexivity.
+Qed.
+Hint Resolve code_le_j_idem.
+
+Lemma code_eq_j_idem (Var : Set) (x : Code Var) : x||x == x.
+Proof. split; auto. Qed.
+Hint Resolve code_eq_j_idem.
+
+Lemma code_le_j_sym (Var : Set) (x y : Code Var) : x||y == y||x.
+Proof. split; auto. Qed.
+
+Lemma code_le_j_assoc (Var : Set) (x y z : Code Var) : x||(y||z) == (x||y)||z.
+Proof.
+  split; auto.
+    apply code_le_j_ub; auto.
+    transitivity (x||y); auto.
+  apply code_le_j_ub; auto.
+  transitivity (y||z); auto.
+Qed.
+
+Lemma code_le_j_bot_left (Var : Set) (x : Code Var) : BOT || x == x.
+Proof. split; auto. Qed.
+Hint Rewrite code_le_j_bot_left : code_simpl.
+
+Lemma code_le_j_bot_right (Var : Set) (x : Code Var) : x || BOT == x.
+Proof. split; auto. Qed.
+Hint Rewrite code_le_j_bot_right : code_simpl.
+
+Lemma code_le_j_top_left (Var : Set) (x : Code Var) : TOP || x == TOP.
+Proof. split; auto. Qed.
+Hint Rewrite code_le_j_top_left : code_simpl.
+
+Lemma code_le_j_top_right (Var : Set) (x : Code Var) : x || TOP == TOP.
+Proof. split; auto. Qed.
+Hint Rewrite code_le_j_top_right : code_simpl.
+
+(** ** Reasoning with extensionality *)
+
+(*
+Ltac abstract M x :=
+  match m with
+  | x => code_ap code_i x
+  | code_ap ?M1 ?M2 =>
+    let code_ap N1 _ := abstract M1 x in
+    let code_ap N2 _ := abstract M2 x in
+    code_ap (code_ap (code_ap code_s N1) N2) x
+  | _ => code_ap code_k x
+  end.
+
+Ltac beta_subs :=
+  match goal with
+  | beta x y
+*)
+
+Lemma code_le_extensionality (Var : Set) (x x' : Code Var) :
+  (forall y, x * y [= x' * y) -> x [= x'.
+Proof.
+  unfold code_le; intros H Var' c f Hconv.
+  (* TODO implement via abstraction algorithm *)
+Admitted.
+
+Lemma code_eq_extensionality (Var : Set) (x x' : Code Var) :
+  (forall y, x * y == x' * y) -> x == x'.
+Proof.
+  intro H; split; apply code_le_extensionality; apply H.
+Qed.
+
+Tactic Notation "eta_expand" :=
+  let x := fresh in
+  match goal with
+  | [|- _ [= _] => apply code_le_extensionality; intro x
+  | [|- _ == _] => apply code_eq_extensionality; intro x
+  end.
+
+Tactic Notation "eta_expand" "as" ident(x) :=
+  match goal with
+  | [|- _ [= _] => apply code_le_extensionality; intro x
+  | [|- _ == _] => apply code_eq_extensionality; intro x
+  end.
+
+Tactic Notation "eta_expand" "in" hyp(H) :=
+  eapply code_le_ap_left in H; beta_reduce in H.
+
+Ltac beta_eta :=
+  beta_reduce; auto
+  || eta_expand; beta_reduce; auto
+  || eta_expand; eta_expand; beta_reduce; auto
+  || eta_expand; eta_expand; eta_expand; beta_reduce; auto.
+
+Lemma code_eq_ap_top (Var : Set) (x : Code Var) : TOP * x == TOP.
+Proof.
+  split; auto.
+  unfold code_le, conv; intros Var' c f H.
+  rewrite (pi_top (K * TOP)); beta_simpl; auto.
+Qed.
+Hint Rewrite code_eq_ap_top : code_simpl.
+
+Lemma code_eq_ap_bot (Var : Set) (x : Code Var) : BOT * x == BOT.
+Proof.
+  split; auto.
+  unfold code_le, conv; intros Var' c f H.
+Admitted.
+Hint Rewrite code_eq_ap_bot : code_simpl.
+
+(** ** Reasoning about closed terms *)
+
+(** A term is closed if it has no variables.
+    In proving [x [= y], it will sometimes be easier to consider only
+    closing variable assignments [f : Var -> Code Empty_set].
+    Thus we introduce an equivalent definition of [x [= y]. *)
+
+Definition code_le_empty {Var : Set} (x y : Code Var) :=
+  let Var' := Empty_set in
+  forall (c : Code Var') (f : Var -> Code Var'),
+  conv (c * (x @ f)) -> conv (c * (y @ f)).
+
+Lemma code_le_empty_complete (Var : Set) (x x' : Code Var) :
+  x [= x' -> code_le_empty x x'.
+Proof.
+  unfold code_le, code_le_empty; intros; auto.
+Qed.
+
+Lemma code_le_empty_sound (Var : Set) (x x' : Code Var) :
+  code_le_empty x x' -> x [= x'.
+Proof.
+  unfold code_le; intros H Var' c f Hconv.
+Admitted.
+
+Theorem code_le_empty_equiv (Var : Set) (x x' : Code Var) :
+  x [= x' <-> code_le_empty x x'.
+Proof.
+  split; [apply code_le_empty_complete | apply code_le_empty_sound].
+Qed.
+
+(** ** Head-normalized versions of convergence and ordering  *)
+
+Fixpoint code_apply {Var : Set} (x : Code Var) (ys : list (Code Var)) :
+  Code Var :=
+  match ys with
+  | nil => x
+  | (y ::ys')%list => code_apply (x * y) ys'
+  end.
+
+Notation "x ** y" := (code_apply x y)%code : code_scope.
+
+Fixpoint code_tuple {Var : Set} (ys : list (Code Var)) : Code Var :=
+  match ys with
+  | nil => I
+  | (y :: ys')%list => code_tuple ys' o (C * I * y)
+  end.
+
+Lemma beta_tuple_apply (Var : Set) (ys : list (Code Var)) :
+  forall x : Code Var, beta (code_tuple ys * x) (x ** ys).
+Proof.
+  induction ys; simpl; auto; intro x.
+  rewrite beta_b.
+  rewrite beta_c.
+  rewrite beta_i.
+  auto.
+Qed.
+Hint Resolve beta_tuple_apply.
+
+Lemma beta_apply_tuple (Var : Set) (ys : list (Code Var)) :
+  forall x : Code Var, beta (x ** ys) (code_tuple ys * x).
+Proof.
+  induction ys; simpl; auto; intro x.
+  rewrite beta_b.
+  rewrite beta_c.
+  rewrite beta_i.
+  auto.
+Qed.
+Hint Resolve beta_apply_tuple.
+
+Definition code_le_apply {Var : Set} (x x' : Code Var) : Prop :=
+  forall (Var' : Set) (ys : list (Code Var')) (f : Var -> Code Var'),
+  conv ((x @ f) ** ys) -> conv ((x' @ f) ** ys).
+
+Lemma code_le_apply_complete (Var : Set) (x x' : Code Var) :
+  x [= x' -> code_le_apply x x'.
+Proof.
+  unfold code_le; intros H Var' ys f Hconv.
+  rewrite beta_apply_tuple; apply H.
+  rewrite beta_tuple_apply; auto.
+Qed.
+
+Lemma code_le_apply_sound (Var : Set) (x x' : Code Var) :
+  code_le_apply x x' -> x [= x'.
+Proof.
+  unfold code_le; intros H Var' c f Hconv.
+  assert (forall (ys : list (Code Var')),
+    conv ((x @ f) ** ys) -> conv ((x' @ f) ** ys)) as H'; auto; clear H.
+  set (y := x @ f) in *; set (y' := x' @ f) in *.
+  inversion Hconv; simpl; auto.
+Admitted.
+
+Theorem code_le_apply_equiv (Var : Set) (x x' : Code Var) :
+  x [= x' <-> code_le_apply x x'.
+Proof.
+  split; [apply code_le_apply_complete | apply code_le_apply_sound].
+Qed.
