src/LeastFixedPoint.v
@@ -1,0 +1,13 @@
+(** * Reasoning about least fixed points *)
+
+Require Import Coq.Program.Basics.
+Require Import Coq.Setoids.Setoid.
+Require Import Coq.Classes.RelationClasses.
+Require Import Coq.Classes.Morphisms.
+Require Export InformationOrdering.
+Open Scope code_scope.
+
+Lemma Y_lfp (Var : Set) (f b : Code Var) :
+  (forall x, x [= b -> f * x [= b) -> Y * f [= b.
+Proof.
+Admitted.
